Strata/Languages/Boogie/Expressions.lean
@@ -17,11 +17,11 @@ open Std (ToFormat Format format)
 
 abbrev Expression : Imperative.PureExpr :=
    { Ident := BoogieIdent,
-     Expr := Lambda.LExpr Lambda.LMonoTy BoogieIdent,
+     Expr := Lambda.LExpr Lambda.LMonoTy Visibility,
      Ty := Lambda.LTy,
-     TyEnv := @Lambda.TEnv BoogieIdent,
-     EvalEnv := Lambda.LState BoogieIdent
-     EqIdent := instDecidableEqBoogieIdent }
+     TyEnv := @Lambda.TEnv Visibility,
+     EvalEnv := Lambda.LState Visibility
+     EqIdent := inferInstanceAs (DecidableEq (Lambda.Identifier _))}
 
 instance : Imperative.HasVarsPure Expression Expression.Expr where
   getVars := Lambda.LExpr.LExpr.getVars
